rename theories under compiler/proofs
removed labelClosuresTheory since it was tiny and justifiably
incorporable in toBytecodeProofsTheory.

compiler/proofs/toBytecodeProofsScript.sml
@@ -1,7 +1,7 @@
 open HolKernel bossLib boolLib boolSimps SatisfySimps listTheory rich_listTheory pairTheory pred_setTheory finite_mapTheory alistTheory relationTheory arithmeticTheory sortingTheory lcsymtacs quantHeuristicsLib quantHeuristicsLibAbbrev
-open miscTheory miscLib CompilerLibTheory CompilerPrimitivesTheory IntLangTheory ToBytecodeTheory compilerTerminationTheory intLangTheory bytecodeTerminationTheory evaluateEquationsTheory expToCexpTheory pmatchTheory labelClosuresTheory bytecodeEvalTheory bytecodeExtraTheory
+open miscTheory miscLib CompilerLibTheory CompilerPrimitivesTheory IntLangTheory ToBytecodeTheory compilerTerminationTheory intLangExtraTheory toIntLangProofsTheory bytecodeTerminationTheory bytecodeEvalTheory bytecodeExtraTheory
 val _ = numLib.prefer_num()
-val _ = new_theory "compileCorrectness"
+val _ = new_theory "toBytecodeProofs"
 
 (* TODO: move? *)
 val with_same_refs = store_thm("with_same_refs",
@@ -1916,14 +1916,6 @@ val compile_bindings_thm = store_thm("compile_bindings_thm",
   rpt AP_TERM_TAC >> rpt AP_THM_TAC >>
   simp[FUN_EQ_THM])
 
-val code_env_cd_def = Define`
-  code_env_cd code (x,(l,ccenv,ce),(az,b)) ⇔
-    good_cd (x,(l,ccenv,ce),(az,b)) ∧
-    ∃cs bc0 cc bc1.
-      ((compile (MAP CTEnv ccenv) (TCTail az 0) 0 cs b).out = cc ++ cs.out) ∧
-      EVERY (combin$C $< cs.next_label o dest_Label) (FILTER is_Label bc0) ∧ l < cs.next_label ∧
-      (code = bc0 ++ Label l :: (REVERSE cc) ++ bc1)`
-
 val Cenv_bs_bind_fv = store_thm("Cenv_bs_bind_fv",
   ``∀cenv ccenv benv bve ret bvs a st fenv defs ix recs envs env pp rd bs s vs az e l e'.
     (cenv = MAP CTEnv ccenv) ∧
@@ -2005,6 +1997,20 @@ val Cenv_bs_bind_fv = store_thm("Cenv_bs_bind_fv",
   simp[Once Cv_bv_cases] >> strip_tac >>
   qpat_assum`∀i. i < LENGTH envs ⇒ X`(qspec_then`n - (LENGTH recs + (LENGTH vs + 1))` mp_tac) >>
   simp[] >> strip_tac >> simp[] )
+
+val good_cd_def = Define`
+  good_cd ((ez,nz,ix),(l,cc,recs,envs),az,b) ⇔
+    EVERY (λv. v < ez) envs ∧
+    free_vars b ⊆ count (LENGTH cc) ∧
+    ∃e e'. (cc,(recs,envs),e') = (bind_fv (az,e) nz ix)`
+
+val code_env_cd_def = Define`
+  code_env_cd code (x,(l,ccenv,ce),(az,b)) ⇔
+    good_cd (x,(l,ccenv,ce),(az,b)) ∧
+    ∃cs bc0 cc bc1.
+      ((compile (MAP CTEnv ccenv) (TCTail az 0) 0 cs b).out = cc ++ cs.out) ∧
+      EVERY (combin$C $< cs.next_label o dest_Label) (FILTER is_Label bc0) ∧ l < cs.next_label ∧
+      (code = bc0 ++ Label l :: (REVERSE cc) ++ bc1)`
 
 val compile_val = store_thm("compile_val",
   ``(∀s env exp res. Cevaluate s env exp res ⇒
@@ -4245,5 +4251,460 @@ val compile_val = store_thm("compile_val",
     metis_tac[SUBMAP_TRANS,IS_PREFIX_TRANS]) >>
   strip_tac >- rw[] >>
   rw[] )
+
+val label_closures_thm = store_thm("label_closures_thm",
+  ``(∀ez j e. (no_labs e) ∧ free_vars e ⊆ count ez ⇒
+     let (e',j') = label_closures ez j e in
+     (j' = j + (LENGTH (free_labs ez e'))) ∧
+     (MAP (FST o FST o SND) (free_labs ez e') = (GENLIST ($+ j) (LENGTH (free_labs ez e')))) ∧
+     free_vars e' ⊆ free_vars e ∧
+     all_labs e' ∧ EVERY good_cd (free_labs ez e') ∧
+     syneq_exp ez ez $= e e') ∧
+    (∀ez j es.
+     (no_labs_list es) ∧ free_vars_list es ⊆ count ez ⇒
+     let (es',j') = label_closures_list ez j es in
+     (j' = j + LENGTH (free_labs_list ez es')) ∧
+     (MAP (FST o FST o SND) (free_labs_list ez es') = (GENLIST ($+ j) (LENGTH (free_labs_list ez es')))) ∧
+     free_vars_list es' ⊆ free_vars_list es ∧
+     all_labs_list es' ∧ EVERY good_cd (free_labs_list ez es') ∧
+     EVERY2 (syneq_exp ez ez $=) es es') ∧
+    (∀ez j nz k defs ds0 ls0.
+     (no_labs_defs (ls0 ++ MAP ($, NONE) defs)) ∧
+     free_vars_defs nz (MAP ($, NONE) defs) ⊆ count ez ∧
+     (LENGTH ds0 = k) ∧ (LENGTH defs = nz - k) ∧ k ≤ nz ∧ (LENGTH ls0 = k) ∧
+     syneq_defs ez ez $= (ls0 ++ MAP ($, NONE) defs) (ds0 ++ MAP ($, NONE) defs) (λv1 v2. v1 < nz ∧ (v2 = v1))
+     ⇒
+     let (defs',j') = label_closures_defs ez j nz k defs in
+     (j' = j + LENGTH (free_labs_defs ez nz k defs')) ∧
+     (MAP (FST o FST o SND) (free_labs_defs ez nz k defs') = GENLIST ($+ j) (LENGTH (free_labs_defs ez nz k defs'))) ∧
+     free_vars_defs nz defs' ⊆ free_vars_defs nz (MAP ($, NONE) defs) ∧
+     (LENGTH defs' = LENGTH defs) ∧
+     all_labs_defs defs' ∧
+     EVERY good_cd (free_labs_defs ez nz k defs') ∧
+     syneq_defs ez ez $= (ls0 ++ (MAP ($, NONE) defs)) (ds0 ++ defs') (λv1 v2. v1 < nz ∧ (v2 = v1)))``,
+  ho_match_mp_tac label_closures_ind >>
+  strip_tac >- (rw[] >> rw[syneq_exp_refl]) >>
+  strip_tac >- (rw[] >> rw[syneq_exp_refl]) >>
+  strip_tac >- (
+    ntac 2 gen_tac >>
+    map_every qx_gen_tac[`e1`,`e2`] >>
+    rpt strip_tac >> fs[] >>
+    `free_vars e2 ⊆ count (ez + 1)` by (
+      fsrw_tac[DNF_ss,ARITH_ss][SUBSET_DEF,PRE_SUB1] >>
+      Cases>>fsrw_tac[ARITH_ss][] ) >> fs[] >>
+    qabbrev_tac`p = label_closures ez j e1` >> PairCases_on`p`>>fs[LET_THM] >>
+    qabbrev_tac`q = label_closures (ez+1) (j + LENGTH (free_labs ez p0)) e2` >> PairCases_on`q`>>fs[] >>
+    simp[LIST_EQ_REWRITE] >>
+    conj_tac >- (
+      gen_tac >>
+      Cases_on`x<LENGTH (free_labs ez p0)`>>
+      lrw[EL_APPEND1,EL_APPEND2] ) >>
+    rfs[] >>
+    conj_tac >- (
+      fsrw_tac[DNF_ss,ARITH_ss][SUBSET_DEF,PRE_SUB1] >>
+      Cases >> rw[ADD1] >>
+      res_tac >>
+      disj2_tac >> HINT_EXISTS_TAC >>
+      fsrw_tac[ARITH_ss][] ) >>
+    simp[Once syneq_exp_cases] >>
+    match_mp_tac (MP_CANON (CONJUNCT1 syneq_exp_mono_V)) >>
+    HINT_EXISTS_TAC >>
+    simp[]) >>
+  strip_tac >- (rw[] >> rw[syneq_exp_refl]) >>
+  strip_tac >- (rw[] >> rw[syneq_exp_refl]) >>
+  strip_tac >- (
+    rpt gen_tac >> strip_tac >> strip_tac >>
+    fs[LET_THM,UNCURRY] >>
+    simp[Once syneq_exp_cases] ) >>
+  strip_tac >- (
+    rw[] >> fs[LET_THM] >>
+    rw[Once syneq_exp_cases] >> rfs[]) >>
+  strip_tac >- (
+    rw[] >> fs[LET_THM] >>
+    rw[Once syneq_exp_cases] >> rfs[]) >>
+  strip_tac >- (
+    ntac 2 gen_tac >>
+    map_every qx_gen_tac[`e1`,`e2`] >>
+    rpt strip_tac >> fs[] >>
+    `free_vars e2 ⊆ count (ez + 1)` by (
+      fsrw_tac[DNF_ss,ARITH_ss][SUBSET_DEF,PRE_SUB1] >>
+      Cases>>fsrw_tac[ARITH_ss][] ) >> fs[] >>
+    qabbrev_tac`p = label_closures ez j e1` >> PairCases_on`p`>>fs[LET_THM] >>
+    qabbrev_tac`q = label_closures (ez+1) (j + LENGTH (free_labs ez p0)) e2` >> PairCases_on`q`>>fs[] >>
+    simp[LIST_EQ_REWRITE] >>
+    conj_tac >- (
+      gen_tac >>
+      Cases_on`x<LENGTH (free_labs ez p0)`>>
+      lrw[EL_APPEND1,EL_APPEND2] ) >>
+    rfs[] >>
+    conj_tac >- (
+      fsrw_tac[DNF_ss,ARITH_ss][SUBSET_DEF,PRE_SUB1] >>
+      Cases >> rw[ADD1] >>
+      res_tac >>
+      disj2_tac >> HINT_EXISTS_TAC >>
+      fsrw_tac[ARITH_ss][] ) >>
+    simp[Once syneq_exp_cases] >>
+    match_mp_tac (MP_CANON (CONJUNCT1 syneq_exp_mono_V)) >>
+    HINT_EXISTS_TAC >>
+    simp[]) >>
+  strip_tac >- (
+    rpt strip_tac >>
+    simp[] >>
+    `FILTER (IS_NONE o FST) defs = defs` by (
+      simp[FILTER_EQ_ID] >>
+      fs[FLAT_EQ_NIL,EVERY_MAP] >>
+      fs[EVERY_MEM,FORALL_PROD] >>
+      qx_gen_tac`z` >> rpt strip_tac >>
+      res_tac >> Cases_on`z`>>fs[] ) >>
+    full_simp_tac std_ss [LET_THM] >>
+    full_simp_tac std_ss [FILTER_EQ_ID,LENGTH_MAP] >>
+    qabbrev_tac`p = label_closures_defs ez j (LENGTH defs) 0 (MAP SND defs)` >>
+    PairCases_on`p`>>
+    `no_labs e`by fs[] >>
+    `free_vars e ⊆ count (ez + LENGTH defs)` by (
+      qpat_assum`free_vars X ⊆ Y`mp_tac >>
+      rpt (pop_assum kall_tac) >>
+      fsrw_tac[DNF_ss,ARITH_ss][SUBSET_DEF,LET_THM] >>
+      srw_tac[ARITH_ss][ADD1] >>
+      res_tac >> fsrw_tac[ARITH_ss][] ) >>
+    full_simp_tac std_ss [] >>
+    qabbrev_tac`q = label_closures (ez + LENGTH defs) p1 e` >>
+    PairCases_on`q` >>
+    full_simp_tac std_ss [] >>
+    `MAP ($, NONE) (MAP SND defs) = defs` by (
+      fs[EVERY_MEM] >>
+      lrw[MAP_MAP_o] >>
+      CONV_TAC(RAND_CONV(REWRITE_CONV[Once (CONJUNCT2 (GSYM MAP_ID)),SimpRHS])) >>
+      lrw[MAP_EQ_f,FORALL_PROD] >> res_tac >> fs[]) >>
+    full_simp_tac std_ss [] >>
+    first_x_assum(qspecl_then[`[]`,`[]`]mp_tac) >>
+    simp[syneq_defs_refl,EVERY_MAP] >>
+    fs[LET_THM] >>
+    strip_tac >>
+    fsrw_tac[ETA_ss][] >>
+    rfs[] >> simp[] >>
+    conj_tac >- (
+      lrw[LIST_EQ_REWRITE] >>
+      Cases_on`x < LENGTH (free_labs_defs ez (LENGTH defs) 0 p0)` >>
+      lrw[EL_APPEND1,EL_APPEND2] ) >>
+    conj_tac >- (
+      fsrw_tac[DNF_ss][SUBSET_DEF,MEM_MAP,free_vars_defs_MAP] >>
+      gen_tac >> strip_tac >>
+      disj2_tac >>
+      qexists_tac`m` >>
+      simp[] ) >>
+    simp[Once syneq_exp_cases] >>
+    HINT_EXISTS_TAC >> simp[] >>
+    match_mp_tac (MP_CANON (CONJUNCT1 syneq_exp_mono_V)) >>
+    HINT_EXISTS_TAC >>
+    simp[]) >>
+  strip_tac >- (
+    rpt gen_tac >> strip_tac >> strip_tac >>
+    first_x_assum(qspecl_then[`[]`,`[]`]mp_tac) >>
+    simp[] >>
+    discharge_hyps >- (
+      simp[syneq_defs_refl] >>
+      PairCases_on`def`>>fs[]) >>
+    qabbrev_tac`p = label_closures_defs ez j 1 0 [def]` >>
+    PairCases_on`p` >>
+    full_simp_tac std_ss [] >>
+    strip_tac >>
+    Cases_on`p0`>>fs[]>>
+    Cases_on`t`>>fs[]>>
+    PairCases_on`h`>>PairCases_on`def`>>fs[]>>
+    simp[Once syneq_exp_cases] >> fs[] >>
+    HINT_EXISTS_TAC >>
+    simp[] ) >>
+  strip_tac >- (
+    rw[] >> PairCases_on`x`>>fs[]>>
+    PairCases_on`y`>>fs[]) >>
+  strip_tac >- (
+    ntac 2 gen_tac >>
+    map_every qx_gen_tac[`e`,`es`] >>
+    rpt strip_tac >>
+    qabbrev_tac`p = label_closures ez j e` >> PairCases_on`p`>>fs[LET_THM] >>
+    qabbrev_tac`q = label_closures_list ez (j + LENGTH (free_labs ez p0)) es` >> PairCases_on`q`>>fs[] >>
+    fs[] >>
+    simp[LIST_EQ_REWRITE] >>
+    conj_tac >- (
+      gen_tac >>
+      Cases_on`x<LENGTH (free_labs ez p0)`>>
+      lrw[EL_APPEND1,EL_APPEND2] ) >>
+    rfs[] >>
+    conj_tac >- (
+      fsrw_tac[DNF_ss][SUBSET_DEF] ) >>
+    simp[Once syneq_exp_cases]) >>
+  strip_tac >- (
+    rw[] >> fs[LET_THM] >> rfs[] >>
+    simp[Once syneq_exp_cases] ) >>
+  strip_tac >- (
+    ntac 2 gen_tac >>
+    map_every qx_gen_tac[`p2`,`e1`,`e2`] >>
+    rpt strip_tac >> fs[] >>
+    qabbrev_tac`p = label_closures ez j e1` >> PairCases_on`p`>>fs[LET_THM] >>
+    qabbrev_tac`q = label_closures ez (j + LENGTH (free_labs ez p0)) e2` >> PairCases_on`q`>>fs[] >>
+    simp[LIST_EQ_REWRITE] >>
+    conj_tac >- (
+      gen_tac >> strip_tac >>
+      Cases_on`x < LENGTH (free_labs ez p0)`>>
+      lrw[EL_APPEND1,EL_APPEND2]) >>
+    conj_tac >- (
+      rfs[] >>
+      fsrw_tac[DNF_ss][SUBSET_DEF] ) >>
+    simp[Once syneq_exp_cases]) >>
+  strip_tac >- (
+    ntac 2 gen_tac >>
+    map_every qx_gen_tac[`e1`,`e2`] >>
+    rpt strip_tac >> fs[] >>
+    qabbrev_tac`p = label_closures ez j e1` >> PairCases_on`p`>>fs[LET_THM] >>
+    qabbrev_tac`q = label_closures ez (j + LENGTH (free_labs ez p0)) e2` >> PairCases_on`q`>>fs[] >>
+    simp[LIST_EQ_REWRITE] >>
+    conj_tac >- (
+      gen_tac >> strip_tac >>
+      Cases_on`x < LENGTH (free_labs ez p0)`>>
+      lrw[EL_APPEND1,EL_APPEND2]) >>
+    conj_tac >- (
+      rfs[] >>
+      fsrw_tac[DNF_ss][SUBSET_DEF] ) >>
+    simp[Once syneq_exp_cases]) >>
+  strip_tac >- (
+    ntac 2 gen_tac >>
+    map_every qx_gen_tac[`e1`,`e2`,`e3`] >>
+    rpt strip_tac >> fs[] >>
+    qabbrev_tac`p = label_closures ez j e1` >> PairCases_on`p`>>fs[LET_THM] >>
+    qabbrev_tac`q = label_closures ez (j + LENGTH (free_labs ez p0)) e2` >> PairCases_on`q`>>fs[] >>
+    qabbrev_tac`r = label_closures ez (j + LENGTH (free_labs ez p0) + LENGTH (free_labs ez q0)) e3` >> PairCases_on`r`>>fs[] >>
+    simp[LIST_EQ_REWRITE] >>
+    conj_tac >- (
+      gen_tac >> strip_tac >>
+      Cases_on`x < LENGTH (free_labs ez p0)`>>
+      lrw[EL_APPEND1,EL_APPEND2] >>
+      Cases_on`x < LENGTH (free_labs ez p0) + LENGTH (free_labs ez q0)` >>
+      lrw[EL_APPEND1,EL_APPEND2] ) >>
+    conj_tac >- (
+      rfs[] >>
+      fsrw_tac[DNF_ss,ARITH_ss][SUBSET_DEF,MEM_GENLIST] ) >>
+    simp[Once syneq_exp_cases]) >>
+  strip_tac >- simp[] >>
+  strip_tac >- (
+    rpt strip_tac >>
+    fs[] >>
+    qabbrev_tac`p = label_closures ez j e` >>
+    PairCases_on`p`>>fs[LET_THM] >>
+    qabbrev_tac`q = label_closures_list ez (j + LENGTH (free_labs ez p0)) es` >>
+    PairCases_on`q`>>fs[] >> simp[] >> rfs[] >>
+    conj_tac >- (
+      lrw[LIST_EQ_REWRITE] >>
+      Cases_on`x < LENGTH (free_labs ez p0)`>>
+      lrw[EL_APPEND1,EL_APPEND2] ) >>
+    conj_tac >- (
+      fsrw_tac[DNF_ss][SUBSET_DEF] ) >>
+    fsrw_tac[DNF_ss][SUBSET_DEF] ) >>
+  strip_tac >- (
+    simp[] >> rw[FUNION_FEMPTY_2] >>
+    fs[LENGTH_NIL]) >>
+  rpt gen_tac >> rpt strip_tac >>
+  full_simp_tac (std_ss++ARITH_ss) [] >>
+  last_x_assum mp_tac >>
+  last_x_assum mp_tac >>
+  simp[] >> ntac 2 strip_tac >>
+  Q.PAT_ABBREV_TAC`r = bind_fv X Y Z` >>
+  PairCases_on`r`>>fs[] >>
+  Q.PAT_ABBREV_TAC`ezz:num = az + (X + (Y + 1))` >>
+  qabbrev_tac`p = label_closures ezz (j+1) r3` >>
+  PairCases_on`p` >> full_simp_tac std_ss [] >>
+  qabbrev_tac`q = label_closures_defs ez p1 nz (k+1) defs` >>
+  PairCases_on`q` >> full_simp_tac std_ss [] >>
+  `no_labs r3` by (
+    fs[bind_fv_def,LET_THM,markerTheory.Abbrev_def] ) >>
+  `free_vars r3 ⊆ count ezz` by (
+    fs[bind_fv_def,LET_THM,markerTheory.Abbrev_def] >>
+    first_x_assum(qspec_then`[]`kall_tac) >>
+    qpat_assum`P⇒Q`kall_tac >>
+    fsrw_tac[DNF_ss][SUBSET_DEF] >>
+    srw_tac[ARITH_ss][] >- (
+      qho_match_abbrev_tac`(THE (find_index x ls n)) < y` >>
+      qho_match_abbrev_tac`P (THE (find_index x ls n))` >>
+      ho_match_mp_tac THE_find_index_suff >>
+      simp[Abbr`P`,Abbr`x`,Abbr`ls`,MEM_FILTER,ADD1,MEM_GENLIST,Abbr`n`,Abbr`y`] >>
+      rw[] >>
+      qmatch_abbrev_tac`m < A + B` >>
+      Cases_on`m=A`>>fsrw_tac[ARITH_ss][]>>
+      Cases_on`B=0`>>fsrw_tac[ARITH_ss][]>>
+      fs[LENGTH_NIL_SYM,FILTER_EQ_NIL,EVERY_MEM,QSORT_MEM,markerTheory.Abbrev_def] >>
+      res_tac >> fsrw_tac[ARITH_ss][]) >>
+    qho_match_abbrev_tac`(THE (find_index x ls n)) < y` >>
+    qho_match_abbrev_tac`P (THE (find_index x ls n))` >>
+    ho_match_mp_tac THE_find_index_suff >>
+    `n ≤ nz` by (
+      unabbrev_all_tac >>
+      simp[GSYM ADD1] >>
+      simp[GSYM LESS_EQ] >>
+      qmatch_abbrev_tac`LENGTH (FILTER P ls) < nz` >>
+      `nz = LENGTH ls` by rw[Abbr`ls`] >> pop_assum SUBST1_TAC >>
+      match_mp_tac LENGTH_FILTER_LESS >>
+      simp[Abbr`P`,Abbr`ls`,EXISTS_MEM,MEM_GENLIST] >>
+      qexists_tac`LENGTH ls0` >>
+      simp[] ) >>
+    reverse conj_tac >- (
+      unabbrev_all_tac >>
+      simp[MEM_MAP,MEM_FILTER,sortingTheory.QSORT_MEM] >>
+      qexists_tac`v` >> simp[] ) >>
+    simp[Abbr`P`,Abbr`y`] >>
+    qx_gen_tac`m`>>strip_tac >>
+    qmatch_abbrev_tac`m + n < l1 + l2` >>
+    `l2 = LENGTH ls + 1` by rw[Abbr`l2`,Abbr`ls`] >> rw[] >>
+    qsuff_tac`n ≤ l1 + 1` >- DECIDE_TAC >>
+    simp[Abbr`n`]) >>
+  full_simp_tac std_ss [LET_THM] >>
+  Q.PAT_ABBREV_TAC`cd:def = (SOME X,az,p0)` >>
+  last_x_assum(qspecl_then[`ds0++[cd]`,`ls0++[(NONE,az,b)]`]mp_tac) >>
+  discharge_hyps >- (
+    simp[] >>
+    rator_x_assum`syneq_defs`mp_tac >>
+    simp[Once syneq_exp_cases] >>
+    simp[EVERY_MAP] >> strip_tac >>
+    simp[Once syneq_exp_cases,EVERY_MAP] >>
+    qx_gen_tac`v` >> strip_tac >>
+    first_x_assum(qspec_then`v`mp_tac) >> simp[] >>
+    REWRITE_TAC[GSYM APPEND_ASSOC] >>
+    Cases_on`v < k`>>simp[EL_APPEND1,EL_APPEND2,ADD1,EL_MAP] >- (
+      strip_tac >>
+      ntac 2 (first_x_assum (mp_tac o SYM)) >>
+      ntac 2 strip_tac >>
+      fsrw_tac[ARITH_ss][ADD1] ) >>
+    Cases_on`v=k` >- (
+      simp[Abbr`cd`] >> strip_tac >>
+      simp[syneq_cb_aux_def] >>
+      fsrw_tac[ARITH_ss][ADD1] >>
+      simp[syneq_cb_aux_def] >>
+      conj_asm1_tac >- (
+        fs[bind_fv_def,LET_THM,markerTheory.Abbrev_def] >>
+        simp[EVERY_MEM,MEM_MAP,MEM_FILTER,QSORT_MEM,MEM_FILTER,MEM_GENLIST] >>
+        simp[GSYM LEFT_FORALL_IMP_THM] >>
+        qpat_assum`IMAGE X  Y ⊆ count ez` mp_tac >>
+        simp[SUBSET_DEF,GSYM LEFT_FORALL_IMP_THM] >>
+        srw_tac[DNF_ss,ARITH_ss][NOT_LESS] >>
+        metis_tac[] ) >>
+      qmatch_abbrev_tac`syneq_exp z1 ezz V b p0` >>
+      qsuff_tac`syneq_exp z1 ezz V b r3` >- (
+        strip_tac >>
+        `V = $= O V` by metis_tac[Id_O] >> pop_assum SUBST1_TAC >>
+        match_mp_tac (MP_CANON (CONJUNCT1 syneq_exp_trans)) >>
+        PROVE_TAC[] ) >>
+      qpat_assum`Abbrev(X = bind_fv A Y Z)`mp_tac >>
+      simp[bind_fv_def,markerTheory.Abbrev_def] >> rw[] >>
+      match_mp_tac mkshift_thm >>
+      simp[Abbr`z1`,Abbr`ezz`] >>
+      conj_tac >- simp[Abbr`V`,syneq_cb_V_def] >>
+      reverse conj_tac >- (
+        qpat_assum`IMAGE X Y ⊆ count ez`mp_tac >>
+        simp[SUBSET_DEF,GSYM LEFT_FORALL_IMP_THM] >>
+        srw_tac[DNF_ss,ARITH_ss][NOT_LESS] >>
+        Cases_on`az + nz ≤ x`>>simp[]) >>
+      gen_tac >> strip_tac >>
+      reverse conj_tac >- (
+        rw[] >- (
+          qho_match_abbrev_tac`THE (find_index a w c) < X` >>
+          qunabbrev_tac`X` >>
+          qho_match_abbrev_tac`P (THE (find_index a w c))` >>
+          match_mp_tac THE_find_index_suff >>
+          reverse conj_tac >- (
+            unabbrev_all_tac >>
+            fs[SUBSET_DEF] >>
+            simp[MEM_FILTER,MEM_GENLIST] ) >>
+          simp[Abbr`w`,Abbr`c`,Abbr`P`]) >>
+        qho_match_abbrev_tac`THE (find_index a w c) < X` >>
+        qunabbrev_tac`X` >>
+        qho_match_abbrev_tac`P (THE (find_index a w c))` >>
+        match_mp_tac THE_find_index_suff >>
+        reverse conj_tac >- (
+          unabbrev_all_tac >>
+          simp[MEM_MAP,MEM_FILTER,QSORT_MEM] >>
+          qexists_tac`x`>>simp[]) >>
+        simp[Abbr`w`,Abbr`c`,Abbr`P`]) >>
+      Q.PAT_ABBREV_TAC`envs:num list = MAP X (FILTER Y (QSORT Z A))` >>
+      `¬(x < az + nz) ⇒ MEM (x-(az+nz)) envs` by (
+        simp[Abbr`envs`,MEM_MAP,MEM_FILTER,QSORT_MEM] >>
+        strip_tac >>
+        qexists_tac`x` >> simp[] ) >>
+      Q.PAT_ABBREV_TAC`recs = LENGTH ls0::X` >>
+      `x < az + nz ⇒ MEM (x - az) recs` by (
+        simp[Abbr`recs`,MEM_FILTER,MEM_GENLIST] ) >>
+      simp[Abbr`V`] >>
+      reverse(rw[]) >- (
+        fs[] >>
+        simp[syneq_cb_V_def] >>
+        Q.PAT_ABBREV_TAC`rz = LENGTH (FILTER X Y) + 1` >>
+        Q.ISPECL_THEN[`envs`,`x-(az+nz)`,`rz`]mp_tac find_index_MEM >>
+        simp[] >> disch_then strip_assume_tac >> simp[] >>
+        simp[Abbr`rz`] ) >>
+      simp[syneq_cb_V_def] >> fs[] >>
+      Q.ISPECL_THEN[`recs`,`x-az`,`0:num`]mp_tac find_index_MEM >>
+      simp[] >> disch_then strip_assume_tac >> simp[] >>
+      Cases_on`i=0` >- (
+        simp[] >> fs[Abbr`recs`]) >>
+      simp[] >>
+      qpat_assum`EL X Y = x - def0`mp_tac >>
+      simp[Abbr`recs`,EL_CONS,PRE_SUB1] >>
+      fsrw_tac[ARITH_ss][]) >>
+    lrw[EL_CONS] >>
+    ntac 2 (qpat_assum`X = Y`(mp_tac o SYM)) >>
+    simp[PRE_SUB1,EL_MAP] >>
+    Q.PAT_ABBREV_TAC`p = EL X defs` >>
+    PairCases_on`p` >>
+    simp[syneq_cb_aux_def] >>
+    ntac 2 strip_tac >>
+    fsrw_tac[ARITH_ss][] >> rw[] >> fs[] >>
+    fsrw_tac[ARITH_ss][ADD1] >>
+    `LENGTH defs + (LENGTH ls0 + 1) = nz` by simp[] >>
+    pop_assum SUBST1_TAC >>
+    match_mp_tac (MP_CANON(CONJUNCT1 syneq_exp_mono_V)) >>
+    HINT_EXISTS_TAC >>
+    simp[]) >>
+  simp[] >> strip_tac >>
+  simp[Abbr`cd`,ADD1]>>
+  conj_tac >- (
+    fsrw_tac[ARITH_ss][] >>
+    lrw[LIST_EQ_REWRITE,EL_CONS,ADD1] >>
+    Cases_on`x=0` >> lrw[EL_CONS,PRE_SUB1] >>
+    Cases_on`x < LENGTH (free_labs ezz p0)` >>
+    lrw[EL_APPEND1,EL_APPEND2] >>
+    Cases_on `x-1 < LENGTH (free_labs ezz p0)` >>
+    lrw[EL_APPEND1,EL_APPEND2]) >>
+  conj_tac >- (
+    rev_full_simp_tac std_ss [] >>
+    fsrw_tac[DNF_ss][SUBSET_DEF] ) >>
+  reverse conj_tac >-
+    metis_tac[CONS_APPEND,APPEND_ASSOC] >>
+  simp[good_cd_def] >>
+  conj_tac >- (
+    fs[bind_fv_def,LET_THM,markerTheory.Abbrev_def] >>
+    simp[EVERY_MAP,EVERY_FILTER] >>
+    simp[EVERY_MEM,QSORT_MEM] >>
+    qpat_assum`IMAGE X Y ⊆ count ez` mp_tac >>
+    srw_tac[DNF_ss][SUBSET_DEF] >>
+    res_tac >> fsrw_tac[ARITH_ss][] ) >>
+  conj_tac >- (
+    fs[bind_fv_def,LET_THM,markerTheory.Abbrev_def] >>
+    qpat_assum`free_vars p0 ⊆ X`mp_tac >>
+    simp[SUBSET_DEF] >> strip_tac >>
+    gen_tac >> strip_tac >>
+    first_x_assum(qspec_then`x`mp_tac) >>
+    simp[] >> strip_tac >>
+    Cases_on`v<az`>>fsrw_tac[ARITH_ss][]>>
+    Cases_on`v<az+nz`>>fsrw_tac[ARITH_ss][]>- (
+      qho_match_abbrev_tac`THE (find_index a ls n) < X` >>
+      qho_match_abbrev_tac`P (THE (find_index a ls n))` >>
+      match_mp_tac THE_find_index_suff >>
+      simp[Abbr`ls`,Abbr`P`,Abbr`X`,MEM_FILTER,MEM_GENLIST,Abbr`n`,Abbr`a`,MEM_MAP,QSORT_MEM] ) >>
+    rw[] >>
+    qho_match_abbrev_tac`THE (find_index a ls n) < X` >>
+    qho_match_abbrev_tac`P (THE (find_index a ls n))` >>
+    match_mp_tac THE_find_index_suff >>
+    simp[Abbr`ls`,Abbr`P`,Abbr`X`,MEM_FILTER,MEM_GENLIST,Abbr`n`,Abbr`a`,MEM_MAP,QSORT_MEM] >>
+    HINT_EXISTS_TAC >> simp[] ) >>
+  map_every qexists_tac[`b`,`r3`] >>
+  simp[])
 
 val _ = export_theory ()
