compiler/proofs/intLangExtraScript.sml
@@ -1,6 +1,6 @@
 open HolKernel bossLib boolLib miscLib boolSimps pairTheory listTheory rich_listTheory pred_setTheory finite_mapTheory relationTheory SatisfySimps arithmeticTheory quantHeuristicsLib lcsymtacs
 open miscTheory semanticsExtraTheory CompilerLibTheory CompilerPrimitivesTheory IntLangTheory ToIntLangTheory compilerTerminationTheory
-val _ = new_theory "intLang"
+val _ = new_theory "intLangExtra"
 
 (* TODO: move?*)
 
