compiler/proofs/toIntLangProofsScript.sml
@@ -1,6 +1,6 @@
 open HolKernel bossLib boolLib miscLib boolSimps intLib pairTheory sumTheory listTheory pred_setTheory finite_mapTheory arithmeticTheory alistTheory rich_listTheory lcsymtacs
-open LibTheory SemanticPrimitivesTheory AstTheory terminationTheory semanticsExtraTheory evaluateEquationsTheory miscTheory CompilerLibTheory IntLangTheory ToIntLangTheory compilerTerminationTheory intLangTheory pmatchTheory
-val _ = new_theory "expToCexp"
+open LibTheory SemanticPrimitivesTheory AstTheory terminationTheory semanticsExtraTheory evaluateEquationsTheory miscTheory CompilerLibTheory IntLangTheory ToIntLangTheory compilerTerminationTheory intLangExtraTheory pmatchTheory
+val _ = new_theory "toIntLangProofs"
 val fsd = full_simp_tac std_ss
 
 (* TODO: move? *)
